![](Pasted%20image%2020240423100900.png)
$S_{1}$ loops forever on $s$, since x starts $\leq0$ and is only ever incremented
$S_{2}$ loops forever on $s$ as well, as y increases by a factor 3 each step, while $x$ only increases by a factor $2$

This gives
$\langle S_{1}, s\rangle\nrightarrow$
$\langle S_{2}, s\rangle\not\rightarrow$

As such $S_{1}\sim_{bs}S_{2}$
![](Pasted%20image%2020240423102244.png)
![](Pasted%20image%2020240423102252.png)

$n_{1}=5, n_2=7$

$y=5+1*7=12$
$x = 8$

$y=5+7*\frac{7+1}{2}=5+7*4=33$
Simple example disproves this

![](Pasted%20image%2020240423103033.png)
Big step
$$
\frac
{\langle x:=e_1;S;\textbf{foreach}\ x\ \textbf{in}\ [e_{2},\dots,e_{m}]\ \textbf{do}\ S, s\rangle\rightarrow s'}
{\langle\textbf{foreach}\ x\ \textbf{in}\ [e_{1},\dots,e_{m}]\ \textbf{do}\ S, s\rangle\rightarrow s'}
$$
$$
\frac
{\langle x:=e; S, s\rangle\rightarrow s'}
{\langle\textbf{foreach}\ x\ \textbf{in}\ [e]\ \textbf{do}\ S, s\rangle\rightarrow s'}
$$
Small step
$$
\langle\textbf{foreach}\ x\ \textbf{in}\ [e_{1},\dots,e_{m}]\ \textbf{do}\ S, s\rangle
$$
$$
\Rightarrow\langle x:=e_1;S;\textbf{foreach}\ x\ \textbf{in}\ [e_{2},\dots,e_{m}]\ \textbf{do}\ S, s\rangle s'
$$
$$
\langle\textbf{foreach}\ x\ \textbf{in}\ [e]\ \textbf{do}\ S, s\rangle\Rightarrow\langle x:=e;S,s\rangle
$$
![](Pasted%20image%2020240423105332.png)
1. Injsert picture
2. 
$$\langle S_{7},s\rangle\Rightarrow\langle S_{6};S_{7},s\rangle
\Rightarrow^{*}\langle S_{7},[x\mapsto-102]\rangle\Rightarrow\langle S_{6};S_{7},[x\mapsto-102]\rangle
$$$$
\Rightarrow^{*}\langle S_{7},[x\mapsto204]\rangle\Rightarrow[x\mapsto204]$$
3. 
$$\langle S_{8},s\rangle\Rightarrow\langle S_{6};S_{8},s\rangle
\Rightarrow^{*}\langle S_{8},[x\mapsto-102]\rangle\Rightarrow\langle S_{6};S_{8},[x\mapsto-102]\rangle
$$$$
\Rightarrow^{*}\langle S_{8},[x\mapsto204]\rangle\Rightarrow[x\mapsto204]$$